We are asked to find the value of the integral
$\oint_{\gamma}\left(\frac{3}{z+2}-\frac{1}{z-2i}\right)dz$ along the curve
$\gamma$ given by $\{|z|=5\}$. We can split the integral into two parts:

\begin{align*}
    \oint_{\gamma}\left(\frac{3}{z+2}-\frac{1}{z-2i}\right)dz & =
    \oint_{\gamma}\frac{3}{z+2}dz - \oint_{\gamma}\frac{1}{z-2i}dz
\end{align*}

And evaluate them separately. Since $2i$ and $-2$ are inside the curve
$\gamma$, and $f(z) = c$ is entire for any constant $c$, we can use Cauchy's
integral formula to evaluate the integrals. Recall Cauchy's integral formula:

\begin{align*}
    f(z_0) & = \frac{1}{2\pi i}\oint_{\gamma}\frac{f(z)}{z-z_0}dz
\end{align*}

Which gives us the value of the integral as $2\pi i f(z_0)$. We can rewrite the integral as

\begin{align*}
    \oint_{\gamma}\frac{3}{z+2}dz & = 3\oint_{\gamma}\frac{1}{z+2}dz = 3\cdot 2\pi i = 6\pi i
\end{align*}

The same goes for the second integral:

\begin{align*}
    \oint_{\gamma}\frac{1}{z-2i}dz & = 2\pi i
\end{align*}

And now, we can add them together to get the value of the original integral:

\begin{align*}
    \oint_{\gamma}\left(\frac{3}{z+2}-\frac{1}{z-2i}\right)dz & = 6\pi i - 2\pi i = 4\pi i
\end{align*}